algo now good

theories/Frontend/Elaborator.v
@@ -70,10 +70,10 @@ Fixpoint elaborate (cst : Cst.obj) (ctx : list string) : option exp :=
       | Some a, Some t => Some (a_sigma t a)
       | _, _ => None
       end
-  | Cst.pair c1 c2 s t => 
-      match elaborate c1 ctx, elaborate c2 ctx, elaborate t (s :: ctx) with
-      | Some a1, Some a2, Some b => Some (a_pair a1 a2 b)
-      | _, _, _ => None
+  | Cst.pair c1 t1 c2 s t2 => 
+      match elaborate c1 ctx,  elaborate t1 ctx, elaborate c2 ctx, elaborate t2 (s::ctx) with
+      | Some a1, Some b1, Some a2, Some b2 => Some (a_pair a1 b1 a2 b2)
+      | _, _, _, _ => None
       end
   | Cst.fst c =>
       match elaborate c ctx with
@@ -141,9 +141,10 @@ Inductive user_exp : exp -> Prop :=
      user_exp (a_sigma A B) )
 | user_exp_pair :
   `( user_exp M ->
+     user_exp A ->
      user_exp N ->
      user_exp B ->
-     user_exp (a_pair M N B) )
+     user_exp (a_pair M A N B) )
 | user_exp_fst :
   `( user_exp M ->
      user_exp (a_fst M) )
@@ -206,7 +207,7 @@ Fixpoint cst_variables (cst : Cst.obj) : StrSet.t :=
   | Cst.fn s t c => StrSet.union (cst_variables t) (StrSet.remove s (cst_variables c))
   | Cst.app c1 c2 => StrSet.union (cst_variables c1) (cst_variables c2)
   | Cst.sigma s t c => StrSet.union (cst_variables t) (StrSet.remove s (cst_variables c))
-  | Cst.pair c1 c2 s t => StrSet.union (StrSet.union (cst_variables c1) (cst_variables c2)) (StrSet.remove s (cst_variables t))
+  | Cst.pair c1 t1 c2 s t2 => StrSet.union (StrSet.union (cst_variables c1) (cst_variables t1)) (StrSet.union (cst_variables c2) (StrSet.remove s (cst_variables t2)))
   | Cst.fst c => cst_variables c  
   | Cst.snd c => cst_variables c
   | Cst.prop_eq c1 t c2 => StrSet.union (cst_variables c1) (StrSet.union (cst_variables t) (cst_variables c2))
@@ -226,7 +227,7 @@ Inductive closed_at : exp -> nat -> Prop :=
  | ca_lam : `( closed_at t n -> closed_at b (1+n) -> closed_at (a_fn t b) n )
  | ca_app : `( closed_at a1 n -> closed_at a2 n -> closed_at (a_app a1 a2) n )
  | ca_sigma : `( closed_at t n -> closed_at b (1+n) -> closed_at (a_sigma t b) n )
- | ca_pair : `( closed_at a1 n -> closed_at a2 n -> closed_at b (1+n) -> closed_at (a_pair a1 a2 b) n )
+ | ca_pair : `( closed_at a1 n -> closed_at b1 n -> closed_at a2 n -> closed_at b2 (1+n) -> closed_at (a_pair a1 b1 a2 b2) n )
  | ca_fst : `( closed_at a n -> closed_at (a_fst a) n )
  | ca_snd : `( closed_at a n -> closed_at (a_snd a) n )
  | ca_eq : `( closed_at t n -> closed_at a1 n -> closed_at a2 n -> closed_at (a_eq t a1 a2) n )
@@ -335,10 +336,12 @@ Proof.
   - (* pair *)
     assert (cst_variables cst1 [<=] StrSProp.of_list ctx) by fsetdec.
     assert (cst_variables cst2 [<=] StrSProp.of_list ctx) by fsetdec.
-    assert (cst_variables cst3 [<=] StrSProp.of_list (s :: ctx)) by (simpl; fsetdec).
+    assert (cst_variables cst3 [<=] StrSProp.of_list ctx) by (simpl; fsetdec).
+    assert (cst_variables cst4 [<=] StrSProp.of_list (s :: ctx)) by (simpl; fsetdec).
     destruct (IHcst1 _ H0) as [ast [-> ?]];
     destruct (IHcst2 _ H1) as [ast' [-> ?]]; mauto.
     destruct (IHcst3 _ H2) as [ast'' [-> ?]]; mauto.
+    destruct (IHcst4 _ H3) as [ast''' [-> ?]]; mauto.
   - (* fst *)
     destruct (IHcst _ H) as [ast [-> ?]]; mauto.
   - (* snd *)
@@ -373,7 +376,7 @@ Proof.
     apply (In_nth _ _ s)  in H.
     destruct H as [? [? ?]].
     mauto.
-Admitted.
+Qed.
 
 Example test_elab : elaborate Cst.nat nil = Some a_nat.
 Proof. reflexivity. Qed.
